Fix linearity in insert, insertB, erase

Hashmap/DHashMap/Basic.lean
@@ -89,19 +89,8 @@ where
   let ⟨i, h⟩ := mkIdx buckets.size hm (hash a)
   let bkt := buckets[i]
   if bkt.contains a then
-    ⟨⟨size, buckets.uset i (bkt.replace a b) h⟩, by simpa [-List.length_pos]⟩
-  else
-    let size'    := size + 1
-    let buckets' := buckets.uset i (AssocList.cons a b bkt) h
-    expandIfNecessary ⟨⟨size', buckets'⟩, by simpa [buckets', -List.length_pos]⟩
-
-@[inline] def insertLinear [BEq α] [Hashable α] (m : Raw₀ α β) (a : α) (b : β a) : Raw₀ α β :=
-  let ⟨⟨size, buckets⟩, hm⟩ := m
-  let ⟨i, h⟩ := mkIdx buckets.size hm (hash a)
-  let bkt := buckets[i]
-  if bkt.contains a then
-    let buckets := buckets.uset i .nil h
-    ⟨⟨size, buckets.uset i (bkt.replace a b) (by simpa [buckets])⟩, by simpa [-List.length_pos, buckets]⟩
+    let buckets' := buckets.uset i .nil h
+    ⟨⟨size, buckets'.uset i (bkt.replace a b) (by simpa [buckets'])⟩, by simpa [-List.length_pos, buckets']⟩
   else
     let size'    := size + 1
     let buckets' := buckets.uset i (AssocList.cons a b bkt) h
@@ -112,7 +101,8 @@ where
   let ⟨i, h⟩ := mkIdx buckets.size hm (hash a)
   let bkt := buckets[i]
   if bkt.contains a then
-    (⟨⟨size, buckets.uset i (bkt.replace a b) h⟩, by simpa [-List.length_pos]⟩, true)
+    let buckets' := buckets.uset i .nil h
+    (⟨⟨size, buckets'.uset i (bkt.replace a b) (by simpa [buckets'])⟩, by simpa [-List.length_pos, buckets']⟩, true)
   else
     let size'    := size + 1
     let buckets' := buckets.uset i (AssocList.cons a b bkt) h
@@ -185,7 +175,8 @@ def erase [BEq α] [Hashable α] (m : Raw₀ α β) (a : α) : Raw₀ α β :=
   let ⟨i, h⟩ := mkIdx buckets.size hb (hash a)
   let bkt := buckets[i]
   if bkt.contains a then
-    ⟨⟨size - 1, buckets.uset i (bkt.erase a) h⟩, by simpa [-List.length_pos]⟩
+    let buckets' := buckets.uset i .nil h
+    ⟨⟨size - 1, buckets'.uset i (bkt.erase a) (by simpa [buckets'])⟩, by simpa [-List.length_pos, buckets']⟩
   else
     ⟨⟨size, buckets⟩, hb⟩
 
@@ -412,9 +403,6 @@ Inserts the mapping into the map, replacing an existing mapping if there is one.
 -/
 @[inline] def insert [BEq α] [Hashable α] (m : DHashMap α β) (a : α) (b : β a) : DHashMap α β :=
   ⟨Raw₀.insert ⟨m.1, m.2.size_buckets_pos⟩ a b, .insert₀ m.2⟩
-
-@[inline] def insertLinear [BEq α] [Hashable α] (m : DHashMap α β) (a : α) (b : β a) : DHashMap α β :=
-  ⟨Raw₀.insertLinear ⟨m.1, m.2.size_buckets_pos⟩ a b, sorry⟩
 
 /--
 If the map contains a mapping for the given key, return the value. Otherwise, compute the value using the
